Add pattern matching role steps to ESPL
The theory can be built, but automation is broken.

data/isabelle/src/ESPLogic/Protocol.thy
@@ -112,13 +112,51 @@ type_synonym lbl = string
 
 datatype notetype = RandGen | State | SessKey
 
-datatype rolestep = Send lbl pattern | Recv lbl pattern | Note lbl notetype pattern
+datatype rolestep = Send lbl pattern
+| Recv lbl pattern
+| Match lbl pattern pattern
+| NotMatch lbl pattern pattern
+| Note lbl notetype pattern
+
+fun sourced_vars :: "rolestep \<Rightarrow> id set"
+where
+  "sourced_vars (Recv _ pt)     = FMV pt"
+| "sourced_vars (Match _ pl _) = FMV pl"
+| "sourced_vars _ = {}"
+
+fun used_vars :: "rolestep \<Rightarrow> id set"
+where
+  "used_vars (Send     _ msg)   = FMV msg"
+| "used_vars (Recv     _ _)     = {}"
+| "used_vars (Match    _ _ pr)  = FMV pr"
+| "used_vars (NotMatch _ _ pr)  = FMV pr"
+| "used_vars (Note     _ _ msg) = FMV msg"
+
+fun FV_rolestep :: "rolestep \<Rightarrow> varid set"
+where
+  "FV_rolestep (Send     _   pt)    = FV pt"
+| "FV_rolestep (Recv     _   pt)    = FV pt"
+| "FV_rolestep (Match    _   p1 p2) = FV p1 \<union> FV p2"
+| "FV_rolestep (NotMatch _   _  p2) = FV p2"  (* sic! *)
+| "FV_rolestep (Note     _ _ pt)    = FV pt"
+
+fun FAV_rolestep :: "rolestep \<Rightarrow> id set"
+where
+  "FAV_rolestep (Send     _   pt)    = FAV pt"
+| "FAV_rolestep (Recv     _   pt)    = FAV pt"
+| "FAV_rolestep (Match    _   p1 p2) = FAV p1 \<union> FAV p2"
+| "FAV_rolestep (NotMatch _   _  p2) = FAV p2"  (* sic! ??? *)
+| "FAV_rolestep (Note     _ _ pt)    = FAV pt"
 
 fun stepPat :: "rolestep \<Rightarrow> pattern"
 where
-  "stepPat (Send lbl msg)    = msg"
-| "stepPat (Recv lbl msg)    = msg"
+  "stepPat (Send lbl msg) = msg"
+| "stepPat (Recv lbl msg) = msg"
 | "stepPat (Note lbl ty msg) = msg"
+
+fun matchPats :: "rolestep \<Rightarrow> (pattern \<times> pattern)"
+where
+  "matchPats (Match lbl p1 p2) = (p1, p2)"
 
 fun noteType :: "rolestep \<Rightarrow> notetype"
 where
@@ -126,18 +164,28 @@ where
 
 fun sendStep :: "rolestep \<Rightarrow> bool"
 where
-  "sendStep (Send lbl    msg) = True"
-| "sendStep (Recv lbl    msg) = False"
-| "sendStep (Note lbl ty msg) = False"
+  "sendStep (Send lbl msg) = True"
+| "sendStep _             = False"
 
 fun noteStep :: "rolestep \<Rightarrow> bool"
 where
-  "noteStep (Send lbl    msg) = False"
-| "noteStep (Recv lbl    msg) = False"
-| "noteStep (Note lbl ty msg) = True"
+  "noteStep (Note lbl ty msg) = True"
+| "noteStep _                 = False"
 
+fun recvStep :: "rolestep \<Rightarrow> bool"
+where
+  "recvStep (Recv lbl v) = True"
+| "recvStep _            = False"
 
-abbreviation recvStep where "recvStep x \<equiv> \<not>sendStep x \<and> \<not> noteStep x"
+fun matchStep :: "rolestep \<Rightarrow> bool"
+where
+  "matchStep (Match lbl p1 p2) = True"
+| "matchStep _                 = False"
+
+fun notMatchStep :: "rolestep \<Rightarrow> bool"
+where
+  "notMatchStep (NotMatch lbl p1 p2) = True"
+| "notMatchStep _                    = False"
 
 lemma sendStepD [simp]:
   assumes inStep: "sendStep step"
@@ -148,9 +196,23 @@ qed auto
 
 lemma recvStepD [simp]:
   assumes inStep: "recvStep step"
-  shows "\<exists> l pt. step = (Recv l pt)"
+  shows "\<exists> l v. step = (Recv l v)"
 using inStep
 proof(cases step)
+qed auto
+
+lemma matchStepD [simp]:
+  assumes inStep: "matchStep step"
+  shows "\<exists> l p1 p2. step = (Match l p1 p2)"
+using inStep
+proof (cases step)
+qed auto
+
+lemma notMatchStepD [simp]:
+  assumes inStep: "notMatchStep step"
+  shows "\<exists> l p1 p2. step = (NotMatch l p1 p2)"
+using inStep
+proof (cases step)
 qed auto
 
 lemma noteStepD [simp]:
@@ -160,23 +222,28 @@ using inStep
 proof(cases step)
 qed auto
 
+lemma note_source:
+  assumes "v \<in> sourced_vars s"
+  shows "\<not> noteStep s"
+proof
+  assume "noteStep s"
+  hence "sourced_vars s = {}" by (auto dest: noteStepD)
+  thus "False" using assms by simp
+qed
+
 
 type_synonym "role" = "rolestep list"
 
-fun recv_before :: "id set \<Rightarrow> role \<Rightarrow> bool"
+fun source_before_use :: "id set \<Rightarrow> role \<Rightarrow> bool"
 where
-  "recv_before bound []                = True"
-| "recv_before bound (Recv _ msg # xs) = 
-     recv_before (bound \<union> FMV msg) xs"
-| "recv_before bound (Note _ _ msg # xs) =
-     ((\<forall> v. v \<in> FMV msg \<longrightarrow> v \<in> bound) \<and>  recv_before bound xs)"
-| "recv_before bound (Send _ msg # xs) =
-     ((\<forall> v. v \<in> FMV msg \<longrightarrow> v \<in> bound) \<and>  recv_before bound xs)"
-
+  "source_before_use bound [] = True"
+| "source_before_use bound (step # xs) =
+    ((used_vars step \<subseteq> bound)
+    \<and> source_before_use (bound \<union> sourced_vars step) xs)"
 
 locale wf_role =
   distinct_list R for R :: "role" +
-  assumes recv_msgVar_first [iff]: "recv_before {} R"
+  assumes source_msgVar_first [iff]: "source_before_use {} R"
 
   
 subsubsection{* Protocols *}
@@ -192,80 +259,44 @@ subsection{* Properties *}
 
 subsubsection{* Well-Formed Roles *}
 
-lemma recv_before_sent_distinct_Send_FV:
-  "\<lbrakk>  recv_before V (R@ Send lbl pt # R'); 
-      distinct (R @ Send lbl pt # R');
-      v \<in> FMV pt; v \<notin> V 
+lemma source_before_use_distinct:
+  "\<lbrakk>  source_before_use V (R @ step # R');
+      distinct (R @ step # R');
+      v \<in> used_vars step; v \<notin> V
    \<rbrakk> \<Longrightarrow>
-   \<exists> lbl' pt'. Recv lbl' pt' \<in> set R \<and> v \<in> FMV pt'"
-proof(induct R arbitrary: V)
-  case (Cons step R) note IH = this show ?case
-    proof(cases step)
-      case (Send lbl pt) thus ?thesis using IH by auto
+   (\<exists> step'. step' \<in> set R \<and> v \<in> sourced_vars step')"
+proof (induct R arbitrary: V)
+  case (Cons step R)
+    note IH = this show ?case
+    proof (cases step)
+      case (Send lbl pt) thus ?thesis using IH by fastforce
     next
-      case (Recv lbl pt) thus ?thesis using IH by (auto, fast)
+      case (Recv lbl v') thus ?thesis using IH by fastforce
     next
-      case (Note lbl ty pt) thus ?thesis using IH by auto
+      case (Match lbl ptl ptr) thus ?thesis using IH by fastforce
+    next
+      case (NotMatch lbl ptl ptr) thus ?thesis using IH by fastforce
+    next
+      case (Note lbl ty pt) thus ?thesis using IH by fastforce
     qed
-qed simp
+qed auto
 
-lemma recv_before_note_distinct_Note_FV:
-  "\<lbrakk>  recv_before V (R@ Note lbl ty pt # R'); 
-      distinct (R @ Note lbl ty pt # R');
-      v \<in> FMV pt; v \<notin> V 
-   \<rbrakk> \<Longrightarrow>
-   \<exists> lbl' pt'. Recv lbl' pt' \<in> set R \<and> v \<in> FMV pt'"
-proof(induct R arbitrary: V)
-  case (Cons Note R) 
-  note IH = this show ?case
-    proof(cases Note)
-      case (Send lbl pt) thus ?thesis using IH by auto
-    next
-      case (Recv lbl pt) thus ?thesis using IH by (auto, fast)
-    next
-      case (Note lbl ty pt) thus ?thesis using IH by auto
-    qed
-qed simp
-
-
-lemma (in wf_role) Send_FV:
-  assumes Send: "Send lbl pt \<in> set R" (is "?send \<in> set R")
-      and FV:   "v \<in> FMV pt"
-  shows "\<exists> lbl' pt'. listOrd R (Recv lbl' pt') (Send lbl pt) \<and> v \<in> FMV pt'" 
-using Send 
+lemma (in wf_role) source_use_ord:
+  assumes useR: "ustep \<in> set R"
+      and useV: "v \<in> used_vars ustep"
+    shows "\<exists> sstep. v \<in> sourced_vars sstep \<and> listOrd R sstep ustep" (is "\<exists> sstep. ?source sstep")
+using useR
 proof -
-  let ?send = "Send lbl pt"
-    and "\<exists> lbl' pt'. ?received lbl' pt'" = ?thesis
-  assume "?send \<in> set R" then
-  obtain ys zs 
-    where split: "R = ys @ ?send # zs" by (blast dest!: split_list)
-  moreover have "distinct R" and "recv_before {} R" by auto
-  ultimately obtain lbl' pt' where "Recv lbl' pt' \<in> set ys" 
-                                and "v \<in> FMV pt'"
-             by (fastforce dest!: recv_before_sent_distinct_Send_FV intro!: FV)
-  hence "?received lbl' pt'" using split by auto
+  assume "ustep \<in> set R"
+  then obtain ys zs 
+    where split: "R = ys @ ustep # zs" by (blast dest!: split_list)
+  moreover have "distinct R" and "source_before_use {} R" by auto
+  ultimately obtain sstep where "v \<in> sourced_vars sstep" and "sstep \<in> set ys"
+             by (fastforce dest!: source_before_use_distinct intro!: useV)
+  hence "?source sstep" using split by fastforce
   thus ?thesis by blast
 qed
 
-
-lemma (in wf_role) Note_FV:
-  assumes Note: "Note lbl ty pt \<in> set R" (is "?note \<in> set R")
-      and FV:   "v \<in> FMV pt"
-  shows "\<exists> lbl' pt'. listOrd R (Recv lbl' pt') (Note lbl ty pt) \<and> v \<in> FMV pt'" 
-using Note
-proof -
-  let ?send = "Note lbl ty pt"
-    and "\<exists> lbl' pt'. ?received lbl' pt'" = ?thesis
-  assume "?note \<in> set R" then
-  obtain ys zs 
-    where split: "R = ys @ ?note # zs" by (blast dest!: split_list)
-  moreover have "distinct R" and "recv_before {} R" by auto
-  ultimately obtain lbl' pt' where "Recv lbl' pt' \<in> set ys" 
-                                and "v \<in> FMV pt'"
-             by (fastforce dest!: recv_before_note_distinct_Note_FV intro!: FV)
-  hence "?received lbl' pt'" using split by auto
-  thus ?thesis by blast
-qed
 
 lemma FV_FAV_conv[iff]:
   "(a \<in> FAV pt) = ((AVar a) \<in> FV pt)"
@@ -287,7 +318,7 @@ qed auto
 
 definition aVars:: "role \<Rightarrow> varid set"
 where
-  "aVars role = foldr (\<lambda> st se. (AVar ` FAV (stepPat st)) \<union> se) role {}"
+  "aVars role = foldr (\<lambda> st se. (AVar ` FAV_rolestep st) \<union> se) role {}"
 
 lemma aVars_singleton[iff]:
   "AVar a \<notin> aVars []"
@@ -296,11 +327,11 @@ by(fastforce simp add: aVars_def)
 lemma aVars_Nil [iff]: "aVars [] = {}"
   by (auto simp: aVars_def)
 
-lemma aVars_Cons [simp]: "aVars (s#xs) = (AVar ` FAV (stepPat s) \<union> aVars xs)"
+lemma aVars_Cons [simp]: "aVars (s#xs) = (AVar ` FAV_rolestep s \<union> aVars xs)"
   by (auto simp: aVars_def)
 
 lemma aVars_FAV_conv:
-  "(AVar a \<in> aVars R) = (\<exists> s \<in> set R. \<exists> pt. (stepPat s = pt \<and> a \<in> FAV pt))"
+  "(AVar a \<in> aVars R) = (\<exists> s \<in> set R. a \<in> FAV_rolestep s)"
 by (induct R) ( fastforce simp add: aVars_def)+
 
 
