data/isabelle/src/ESPLogic/ExplicitModel.thy
@@ -149,6 +149,22 @@ where
           \<rbrakk>
           \<Longrightarrow> (t @ [Step (i, Recv l pt)], r(i \<mapsto> (done @ [Recv l pt], todo, skipped)), s) \<in> reachable P"
 
+| match: "\<lbrakk> (t, r, s) \<in> reachable P;
+            r i = Some (done, Match l ptl ptr # todo, skipped);
+            Some ml = inst s i ptl;
+            Some mr = inst s i ptr;
+            ml = mr
+          \<rbrakk>
+          \<Longrightarrow> (t @ [Step (i, Match l ptl ptr)], r(i \<mapsto> (done @ [Match l ptl ptr], todo, skipped)), s) \<in> reachable P"
+
+| notMatch: "\<lbrakk> (t, r, s) \<in> reachable P;
+               r i = Some (done, NotMatch l ptl ptr # todo, skipped);
+               Some ml = inst s i ptl;
+               Some mr = inst s i ptr;
+               ml \<noteq> mr
+             \<rbrakk>
+             \<Longrightarrow> (t @ [Step (i, NotMatch l ptl ptr)], r(i \<mapsto> (done @ [NotMatch l ptl ptr], todo, skipped)), s) \<in> reachable P"
+
 | hash:  "\<lbrakk> (t, r, s) \<in> reachable P;
             m \<in> knows t;
             Hash m \<notin> knows t
@@ -187,7 +203,7 @@ begin
     [ OF reachable
     , rule_format
     , consumes 0
-    , case_names init compr skip lkr send recv hash tuple encr decr
+    , case_names init compr skip lkr send recv match notMatch hash tuple encr decr
     ]
 end
 
@@ -342,6 +358,15 @@ lemma recv_notin_skipped [iff]:
   "Recv l pt \<notin> skipped"
  by (auto dest!: note_in_skipped)
 
+lemma match_notin_skipped [iff]:
+  "Match l ptl ptr \<notin> skipped"
+  by (auto dest!: note_in_skipped)
+
+lemma notMatch_notin_skipped [iff]:
+  "NotMatch l ptl ptr \<notin> skipped"
+  by (auto dest!: note_in_skipped)
+
+
 lemma in_steps_conv_done_skipped:
   "(i, step) \<in> steps t = 
    (step \<in> set done \<and> step \<notin> skipped)"
@@ -372,13 +397,33 @@ next
       using recv `i = i'` by fastforce
   qed auto
 next
+  case (match t r s i "done" l ptl ptr todo skipped ml mr i' done' todo' skipped')
+  thus ?case
+  proof(cases "i = i'")
+    case True
+    then interpret thread:
+        reachable_thread P t r s i "done" "Match l ptl ptr # todo" skipped'
+        using match by unfold_locales auto
+      show ?thesis using match `i = i'` by fastforce 
+  qed auto
+next
+  case (notMatch t r s i "done" l ptl ptr todo skipped ml mr i' done' todo' skipped')
+  thus ?case
+  proof(cases "i = i'")
+    case True
+    then interpret thread:
+        reachable_thread P t r s i "done" "NotMatch l ptl ptr # todo" skipped'
+        using notMatch by unfold_locales auto
+      show ?thesis using notMatch `i = i'` by fastforce 
+  qed auto
+next
   case (compr t r s i "done" l ty pt todo skipped m i' done' todo' skipped')  
   thus ?case
   proof(cases "i = i'")
     case True
     thus ?thesis using compr `i = i'`
     proof(cases "step = Note l ty pt")
-       case True
+      case True
       interpret thread:
         reachable_thread P t r s i "done" "Note l ty pt # todo" skipped'
         using compr  `i = i'` by unfold_locales auto
@@ -417,11 +462,38 @@ proof(induct arbitrary: i "done" todo skipped rule rule: reachable_induct)
     thus "?case" by fastforce
 qed ((unfold map_upd_Some_unfold)?, auto)+
 
+lemma in_steps_match:
+  "((Match l ptl ptr) \<in> set done) = ((i, Match l ptl ptr) \<in> steps t)"
+using thread_exists
+proof(induct arbitrary: i "done" todo skipped rule rule: reachable_induct)
+  case init
+    thus ?case by fastforce
+qed ((unfold map_upd_Some_unfold)?, auto)+
+
+lemma in_steps_notMatch:
+  "((NotMatch l ptl ptr) \<in> set done) = ((i, NotMatch l ptl ptr) \<in> steps t)"
+using thread_exists
+proof(induct arbitrary: i "done" todo skipped rule rule: reachable_induct)
+  case init
+    thus ?case by fastforce
+qed ((unfold map_upd_Some_unfold)?, auto)+
+
 lemmas send_steps_in_done [elim!] = iffD1[OF in_steps_send, rule_format]
 lemmas send_done_in_steps [elim!] = iffD2[OF in_steps_send, rule_format]
 lemmas recv_steps_in_done [elim!] = iffD1[OF in_steps_recv, rule_format]
 lemmas recv_done_in_steps [elim!] = iffD2[OF in_steps_recv, rule_format]
 
+lemmas match_steps_in_done    [elim!] = iffD1[OF in_steps_match, rule_format]
+lemmas match_done_in_steps    [elim!] = iffD2[OF in_steps_match, rule_format]
+lemmas notMatch_steps_in_done [elim!] = iffD1[OF in_steps_notMatch, rule_format]
+lemmas notMatch_done_in_steps [elim!] = iffD2[OF in_steps_notMatch, rule_format]
+
+lemma not_note_done_in_steps:
+  assumes "step \<in> set done"
+      and "\<not> noteStep step"
+    shows "(i, step) \<in> steps t"
+using assms
+by (cases step, auto)
 
 lemma in_steps_eq_in_done:
   "step \<notin> skipped \<Longrightarrow> ((i, step) \<in> steps t) = (step \<in> set done)" 
@@ -467,6 +539,12 @@ proof(cases step)
 next
   case (Recv l pt)
     thus ?thesis using inSteps by (fastforce dest: in_steps_recv[THEN iffD2])
+next
+  case (Match l ptl ptr)
+    thus ?thesis using inSteps by (fastforce dest: in_steps_match[THEN iffD2])
+next
+  case (NotMatch l ptl ptr)
+    thus ?thesis using inSteps by (fastforce dest: in_steps_notMatch[THEN iffD2])
 next
   case (Note l ty pt)
     thus ?thesis using inSteps by (fastforce simp add: in_steps_conv_done_skipped)
@@ -533,6 +611,26 @@ next
           by fastforce
   qed fastforce
 next
+  case (match t r s i "done" l ptl ptr todo skipped ml mr i' done' todo' skipped')
+  from match show ?case 
+  proof(cases "i = i'")
+    case True
+      interpret this_thread:
+          reachable_thread P t r s i' "done" "Match l ptl ptr # todo'" skipped'
+          using match `i = i'` by unfold_locales auto
+       show ?thesis using match `i = i'` by fastforce
+  qed fastforce
+next
+  case (notMatch t r s i "done" l ptl ptr todo skipped ml mr i' done' todo' skipped')
+  from notMatch show ?case 
+  proof(cases "i = i'")
+    case True
+      interpret this_thread:
+          reachable_thread P t r s i' "done" "NotMatch l ptl ptr # todo'" skipped'
+          using notMatch `i = i'` by unfold_locales auto
+       show ?thesis using notMatch `i = i'` by fastforce
+  qed fastforce
+next
   case (compr t r s i "done" l ty msg todo skipped m i' done' todo' skipped')
   from compr show ?case 
   proof(cases "i = i'")
@@ -576,6 +674,27 @@ using distinct
 using facts
 by(auto dest: in_set_listOrd1 todo_notin_doneD listOrd_done_imp_listOrd_trace in_set_listOrd2  listOrd_append[THEN iffD1] in_steps_conv_done_skipped[THEN iffD1])
 
+lemma listOrd_match_role_imp_listOrd_trace:
+  assumes facts:
+    "(i, step) \<in> steps t"
+    "listOrd (done @ todo) (Match l ptl ptr) step"
+  shows
+    "listOrd t (Step (i, Match l ptl ptr)) (Step (i, step))" 
+using distinct
+using facts
+by(auto dest: in_set_listOrd1 todo_notin_doneD listOrd_done_imp_listOrd_trace in_set_listOrd2  listOrd_append[THEN iffD1] in_steps_conv_done_skipped[THEN iffD1])
+
+lemma listOrd_notMatch_role_imp_listOrd_trace:
+  assumes facts:
+    "(i, step) \<in> steps t"
+    "listOrd (done @ todo) (NotMatch l ptl ptr) step"
+  shows
+    "listOrd t (Step (i, NotMatch l ptl ptr)) (Step (i, step))" 
+using distinct
+using facts
+by(auto dest: in_set_listOrd1 todo_notin_doneD listOrd_done_imp_listOrd_trace in_set_listOrd2  listOrd_append[THEN iffD1] in_steps_conv_done_skipped[THEN iffD1])
+
+
 lemma roleOrd_notSkipped_imp_listOrd_trace:
   assumes facts:
     "(i, step) \<in> steps t"
@@ -613,38 +732,24 @@ lemma inst_AVar_in_knows [iff]:
 
 end (* reachable_state *)
 
-lemma (in reachable_state) send_step_FV:
-  assumes thread_exists: "r i = Some (done, Send l msg # todo, skipped)"
-  and FV: "MVar n \<in> FV msg"
-  shows "\<exists> l' msg'. (i, Recv l' msg') \<in> steps t \<and>  MVar n \<in> FV msg'"
+lemma (in reachable_state) source_step:
+  assumes thread_exists: "r i = Some (done, ustep # todo, skipped)"
+      and useV: "v \<in> used_vars ustep"
+    shows "\<exists> sstep. (i, sstep) \<in> steps t \<and> v \<in> sourced_vars sstep"
 proof -
-  interpret this_thread: reachable_thread P t r s i "done" "Send l msg # todo" skipped
+  interpret this_thread: reachable_thread P t r s i "done" "ustep # todo" skipped
     using thread_exists by unfold_locales auto
-  let ?role = "done @ Send l msg # todo"
-  have "Send l msg \<in> set ?role" by simp
-  then obtain l' msg' 
-    where "listOrd ?role (Recv l' msg') (Send l msg)"
-    and "MVar n \<in> FV msg'"
-    using FV by(fast dest!: this_thread.Send_FV)
-  thus ?thesis using this_thread.distinct
-    by(auto dest: in_set_listOrd1 in_set_listOrd2)
-qed
-
-lemma (in reachable_state) note_step_FV:
-  assumes thread_exists: "r i = Some (done, Note l ty msg # todo, skipped)"
-  and FV: "MVar n \<in> FV msg"
-  shows "\<exists> l' msg'. (i, Recv l'  msg') \<in> steps t \<and>  MVar n \<in> FV msg'"
-proof -
-  interpret this_thread: reachable_thread P t r s i "done" "Note l ty msg # todo" skipped
-    using thread_exists by unfold_locales auto
-  let ?role = "done @ Note l ty msg # todo"
-  have "Note l ty msg \<in> set ?role" by simp
-  then obtain l' msg' 
-    where "listOrd ?role (Recv l' msg') (Note l ty msg)"
-    and "MVar n \<in> FV msg'"
-    using FV by(fast dest!: this_thread.Note_FV)
-  thus ?thesis using this_thread.distinct
-    by(auto dest: in_set_listOrd1 in_set_listOrd2)
+  let ?role = "done @ ustep # todo"
+  have "ustep \<in> set ?role" by simp
+  then obtain sstep
+    where "listOrd ?role sstep ustep"
+    and is_source: "v \<in> sourced_vars sstep"
+    using useV by(fast dest!: this_thread.source_use_ord)
+  hence "sstep \<in> set done" using this_thread.distinct
+    by (auto dest: in_set_listOrd1 in_set_listOrd2)
+  moreover have "\<not> noteStep sstep" using is_source by (metis note_source)
+  ultimately show ?thesis using is_source
+    by (auto intro: this_thread.not_note_done_in_steps)
 qed
 
 
@@ -696,6 +801,20 @@ proof(induct arbitrary: i "done" todo skipped rule: reachable_induct)
     by unfold_locales auto
   show ?case using  `distinct' t` this_thread.distinct
     by(fastforce dest: this_thread.in_steps_in_done)
+next
+  case (match t r s i "done" l ptl ptr todo skipped ml mr)
+  then interpret this_thread:
+    reachable_thread P t r s i "done" "Match l ptl ptr # todo" skipped
+    by unfold_locales auto
+  show ?case using `distinct' t` this_thread.distinct
+    by (fastforce dest: this_thread.in_steps_in_done)
+next
+  case (notMatch t r s i "done" l ptl ptr todo skipped ml mr)
+  then interpret this_thread:
+    reachable_thread P t r s i "done" "NotMatch l ptl ptr # todo" skipped
+    by unfold_locales auto
+  show ?case using `distinct' t` this_thread.distinct
+    by (fastforce dest: this_thread.in_steps_in_done)
 next
   case (send t r s i "done" l msg todo skipped m)
   then interpret this_thread: 
@@ -1102,6 +1221,18 @@ next
   from recv show ?case
     by (fastforce dest: s1.rev_knows_pairParts_closedD)
 next
+  case (match t r s i "done" l ptl ptr todo)
+  then interpret s1: reachable_state P t r s
+    by unfold_locales
+  from match show ?case
+    by (fastforce dest: s1.rev_knows_pairParts_closedD)
+next
+  case (notMatch t r s i "done" l ptl ptr todo)
+  then interpret s1: reachable_state P t r s
+    by unfold_locales
+  from notMatch show ?case
+    by (fastforce dest: s1.rev_knows_pairParts_closedD)
+next
   case (init r s) thus ?case by simp
 next
   case (lkr t r s a)
@@ -1373,6 +1504,116 @@ proof -
         and "Note l' ty' pt' \<notin> skipped'' "
         and "?r' i' = Some (done'', todo'', skipped'')"
         using `r i = Some (done, Recv l pt # todo, skipped)` thread' inDone notSkipped
+        by (cases "i = i'") (fastforce+)
+      hence "?note ?t' ?r' s" using msg chain notSkipped inDone
+        by (fast intro!: decrChain_append)
+      hence "?case" by auto
+    }
+    ultimately show ?case by fastforce
+  next
+    case (match t r s i "done" l ptl ptr todo skipped)
+    hence "?cases m' t r s" 
+      (is "?ik0 \<or> ?hash \<or> ?enc \<or> ?tup \<or> ?chain t r s \<or> ?note t r s \<or> ?keys")
+      by clarsimp
+    moreover
+    { assume "?ik0"   hence "?case" by blast    } moreover
+    { assume "?hash"  hence "?case" by fastforce } moreover
+    { assume "?enc"   hence "?case" by fastforce } moreover
+    { assume "?keys"  hence "?case" by fastforce } moreover
+    { assume "?tup"   hence "?case" by fastforce } moreover
+    { let ?t' = "t@[Step (i, Match l ptl ptr)]"
+      and ?r' = "r(i \<mapsto> (done @ [Match l ptl ptr], todo, skipped))"
+      assume "?chain t r s" then
+      obtain i' done' todo' l' pt' skipped' m
+        where thread': "r i' = Some (done', todo', skipped')"
+        and send: "Send l' pt' \<in> set done'"
+        and msg:  "Some m = inst s i' pt'"
+        and chain:"decrChain [] t {St (i', Send l' pt')} m m'"
+        by auto
+      then interpret th1: reachable_thread P t r s i' done' todo' skipped'
+        using match by unfold_locales auto
+        obtain done'' todo'' skipped''
+        where "Send l' pt' \<in> set done''"
+        and "?r' i' = Some (done'', todo'', skipped'')"
+        using `r i = Some (done, Match l ptl ptr # todo, skipped)` thread' send
+        by (cases "i = i'") (fastforce+)
+      hence "?chain ?t' ?r' s"
+        using chain msg
+        by (fast intro!: decrChain_append)
+      hence "?case" by auto
+    } moreover
+    { let ?t' = "t@[Step (i, Match l ptl ptr)]"
+      and ?r' = "r(i \<mapsto> (done @ [Match l ptl ptr], todo, skipped))"
+      assume "?note t r s" then
+      obtain i' done' todo' skipped' l' ty' pt' m
+        where thread': "r i' = Some (done', todo', skipped')"
+        and inDone: "Note l' ty' pt' \<in> set done'"
+        and notSkipped: "Note l' ty' pt' \<notin> skipped'"
+        and msg: "Some m = inst s i' pt'"
+        and chain: "decrChain [] t {St (i', Note l' ty' pt')} m m'"
+        by auto
+      then interpret th1: reachable_thread P t r s i' done' todo' skipped'
+        using match by unfold_locales auto
+      obtain done'' todo'' skipped''
+        where "Note l' ty' pt' \<in> set done''"
+        and "Note l' ty' pt' \<notin> skipped'' "
+        and "?r' i' = Some (done'', todo'', skipped'')"
+        using `r i = Some (done, Match l ptl ptr # todo, skipped)` thread' inDone notSkipped
+        by (cases "i = i'") (fastforce+)
+      hence "?note ?t' ?r' s" using msg chain notSkipped inDone
+        by (fast intro!: decrChain_append)
+      hence "?case" by auto
+    }
+    ultimately show ?case by fastforce
+  next
+    case (notMatch t r s i "done" l ptl ptr todo skipped)
+    hence "?cases m' t r s" 
+      (is "?ik0 \<or> ?hash \<or> ?enc \<or> ?tup \<or> ?chain t r s \<or> ?note t r s \<or> ?keys")
+      by clarsimp
+    moreover
+    { assume "?ik0"   hence "?case" by blast    } moreover
+    { assume "?hash"  hence "?case" by fastforce } moreover
+    { assume "?enc"   hence "?case" by fastforce } moreover
+    { assume "?keys"  hence "?case" by fastforce } moreover
+    { assume "?tup"   hence "?case" by fastforce } moreover
+    { let ?t' = "t@[Step (i, NotMatch l ptl ptr)]"
+      and ?r' = "r(i \<mapsto> (done @ [NotMatch l ptl ptr], todo, skipped))"
+      assume "?chain t r s" then
+      obtain i' done' todo' l' pt' skipped' m
+        where thread': "r i' = Some (done', todo', skipped')"
+        and send: "Send l' pt' \<in> set done'"
+        and msg:  "Some m = inst s i' pt'"
+        and chain:"decrChain [] t {St (i', Send l' pt')} m m'"
+        by auto
+      then interpret th1: reachable_thread P t r s i' done' todo' skipped'
+        using notMatch by unfold_locales auto
+        obtain done'' todo'' skipped''
+        where "Send l' pt' \<in> set done''"
+        and "?r' i' = Some (done'', todo'', skipped'')"
+        using `r i = Some (done, NotMatch l ptl ptr # todo, skipped)` thread' send
+        by (cases "i = i'") (fastforce+)
+      hence "?chain ?t' ?r' s"
+        using chain msg
+        by (fast intro!: decrChain_append)
+      hence "?case" by auto
+    } moreover
+    { let ?t' = "t@[Step (i, NotMatch l ptl ptr)]"
+      and ?r' = "r(i \<mapsto> (done @ [NotMatch l ptl ptr], todo, skipped))"
+      assume "?note t r s" then
+      obtain i' done' todo' skipped' l' ty' pt' m
+        where thread': "r i' = Some (done', todo', skipped')"
+        and inDone: "Note l' ty' pt' \<in> set done'"
+        and notSkipped: "Note l' ty' pt' \<notin> skipped'"
+        and msg: "Some m = inst s i' pt'"
+        and chain: "decrChain [] t {St (i', Note l' ty' pt')} m m'"
+        by auto
+      then interpret th1: reachable_thread P t r s i' done' todo' skipped'
+        using notMatch by unfold_locales auto
+      obtain done'' todo'' skipped''
+        where "Note l' ty' pt' \<in> set done''"
+        and "Note l' ty' pt' \<notin> skipped'' "
+        and "?r' i' = Some (done'', todo'', skipped'')"
+        using `r i = Some (done, NotMatch l ptl ptr # todo, skipped)` thread' inDone notSkipped
         by (cases "i = i'") (fastforce+)
       hence "?note ?t' ?r' s" using msg chain notSkipped inDone
         by (fast intro!: decrChain_append)
